runapp_payload_offset

steel/Zeta.Steel.LogEntry.fsti
@@ -1,5 +1,18 @@
 module Zeta.Steel.LogEntry
 include Zeta.Steel.LogEntry.Spec
 open Zeta.Steel.Parser
+module U32 = FStar.UInt32
 
 val parser_log_entry : parser spec_parser_log_entry
+
+val runapp_payload_offset
+  (e: log_entry)
+: Pure U32.t
+  (requires (RunApp? e))
+  (ensures (fun res ->
+    let s = spec_serializer_log_entry e in
+    let off = U32.v res in
+    let RunApp pl = e in
+    off <= Seq.length s /\
+    Ghost.reveal pl.rest.ebytes == Seq.slice s off (Seq.length s)
+  ))
