steel/formats/spec/Zeta.Steel.LogEntry.Spec.fst
@@ -1,3 +1,7 @@
 module Zeta.Steel.LogEntry.Spec
 
 let spec_parser_log_entry = Zeta.Formats.LogEntry.parse_log_entry
+
+let spec_serializer_log_entry x =
+  assert (LowParse.Spec.Base.parse Zeta.Formats.LogEntry.parse_log_entry (Zeta.Formats.LogEntry.serialize_log_entry x) == Some (x, Seq.length (Zeta.Formats.LogEntry.serialize_log_entry x))); // pattern requires `LowParse.Spec.Base.parse`
+  Zeta.Formats.LogEntry.serialize_log_entry x
