steel/Zeta.Steel.LogEntry.Spec.fsti
@@ -3,3 +3,4 @@ include Zeta.Steel.LogEntry.Types
 open Zeta.Steel.Parser
 
 val spec_parser_log_entry : spec_parser log_entry
+val spec_serializer_log_entry : spec_serializer spec_parser_log_entry
